examples/MemCacheSubst.v
@@ -1,7 +1,7 @@
 Require Import Ascii Bool String List.
 Require Import Lib.CommonTactics Lib.FMap Lib.ilist Lib.Word Lib.Struct Lib.StringBound.
 Require Import Lts.Syntax Lts.ParametricSyntax Lts.Semantics Lts.Refinement Lts.Notations.
-Require Import Lts.Equiv Lts.Tactics Lts.Specialize Lts.Duplicate Lts.Substitute.
+Require Import Lts.Equiv Lts.Tactics Lts.Specialize Lts.Duplicate Lts.Substitute Lts.ModuleBound.
 Require Import Ex.Msi Ex.MemTypes Ex.RegFile Ex.L1Cache Ex.ChildParent Ex.MemDir.
 Require Import Ex.Fifo Ex.NativeFifo Ex.FifoCorrect Lts.ParametricEquiv Lts.ParametricInline.
 Require Import Ex.MemCache.
@@ -29,8 +29,6 @@ Ltac knodup_regs :=
     match goal with
     | [ |- NoDup (namesOf (getRegInits _)) ] =>
       progress (unfold getRegInits; fold getRegInits)
-    | [ |- NoDup (namesOf (getRegInits (modFromMeta (_ +++ _)))) ] =>
-      rewrite getRegInits_modFromMeta_concat
     | [ |- NoDup (namesOf (_ ++ _)) ] => unfold RegInitT; rewrite namesOf_app
     | [ |- NoDup (_ ++ _) ] => apply NoDup_DisjList; [| |kdisj_regs]
     | [ |- NoDup (namesOf (getRegInits ?m)) ] => unfold_head m
@@ -40,6 +38,12 @@ Ltac knodup_regs :=
     | _ => apply noDup_metaRegs
     | _ => noDup_tac
     end.
+
+Lemma getCalls_flattened:
+  forall m,
+    getCalls (Syntax.Mod (getRegInits m) (getRules m) (getDefsBodies m)) =
+    getCalls m.
+Proof. reflexivity. Qed.
 
 Section Refinement.
   Variables IdxBits TagBits LgNumDatas LgDataBytes: nat.
@@ -70,15 +74,40 @@ Section Refinement.
              (sdms := getDefsBodies nfifos)
              (regs' := getRegInits others)
              (rules' := getRules others)
-             (dms' := getDefsBodies others); admit.
-  
+             (dms' := getDefsBodies others);
+        unfold fifos, nfifos, others; clear fifos nfifos others.
+      + admit. (* PHOAS equivalence *)
+      + admit.
+      + admit.
+      + admit.
+      + admit.
+      + admit.
+      + knodup_regs.
+      + knodup_regs.
+      + knodup_regs.
+      + kdisj_regs.
+      + kdisj_regs.
+      + kdisj_dms.
+      + kdisj_dms.
+      + repeat rewrite getCalls_flattened; kdisj_cms.
+      + repeat rewrite getCalls_flattened; kdisj_cms.
+      + admit. (* DefCallSub for flattened modules *)
+      + admit. (* ValidRegsModules for flattened modules *)
+      + admit.
+      + admit.
+      + admit. (* EquivList *)
+      + admit.
+      + admit.
+
+      + admit. (* Real substitution proof -- from fifos to nativeFifos *)
+
     - apply traceRefines_same_module_structure.
-      + admit. (* knodup_regs. *)
-      + admit. (* knodup_regs. *)
+      + knodup_regs.
+      + knodup_regs.
+      + admit. (* EquivList *)
       + admit.
       + admit.
-      + admit.
-        
+
   Qed.
 
 End Refinement.
